Updating the core theory: Latest Simon s version
git-svn-id: orca@411

C-verifier/src/Midend-IVL/Isabelle-UTP/utils/Pfun.thy
@@ -14,7 +14,8 @@ typedef ('a, 'b) pfun = "UNIV :: ('a \<rightharpoonup> 'b) set" ..
 
 setup_lifting type_definition_pfun
 
-lift_definition pfun_app :: "('a, 'b) pfun \<Rightarrow> 'a \<Rightarrow> 'b" ("_'(_')\<^sub>p" [999,0] 999) is "\<lambda> f x. the (f x)" .
+lift_definition pfun_app :: "('a, 'b) pfun \<Rightarrow> 'a \<Rightarrow> 'b" ("_'(_')\<^sub>p" [999,0] 999) is 
+"\<lambda> f x. if (x \<in> dom f) then the (f x) else undefined" .
 
 lift_definition pfun_upd :: "('a, 'b) pfun \<Rightarrow> 'a \<Rightarrow> 'b \<Rightarrow> ('a, 'b) pfun"
 is "\<lambda> f k v. f(k := Some v)" .
@@ -32,16 +33,19 @@ lift_definition pId_on :: "'a set \<Rightarrow> ('a, 'a) pfun" is "\<lambda> A x
 abbreviation pId :: "('a, 'a) pfun" where
 "pId \<equiv> pId_on UNIV"
 
-lift_definition pdom_res :: "'a set \<Rightarrow> ('a, 'b) pfun \<Rightarrow> ('a, 'b) pfun" (infixl "\<lhd>\<^sub>p" 85) 
+lift_definition pdom_res :: "'a set \<Rightarrow> ('a, 'b) pfun \<Rightarrow> ('a, 'b) pfun" (infixl "\<lhd>\<^sub>p" 85)
 is "\<lambda> A f. restrict_map f A" .
 
-lift_definition pran_res :: "('a, 'b) pfun \<Rightarrow> 'b set \<Rightarrow> ('a, 'b) pfun" (infixl "\<rhd>\<^sub>p" 85) 
+lift_definition pran_res :: "('a, 'b) pfun \<Rightarrow> 'b set \<Rightarrow> ('a, 'b) pfun" (infixl "\<rhd>\<^sub>p" 85)
 is ran_restrict_map .
 
 lift_definition pfun_graph :: "('a, 'b) pfun \<Rightarrow> ('a \<times> 'b) set" is map_graph .
 
 lift_definition graph_pfun :: "('a \<times> 'b) set \<Rightarrow> ('a, 'b) pfun" is graph_map .
 
+lift_definition pfun_entries :: "'k set \<Rightarrow> ('k \<Rightarrow> 'v) \<Rightarrow> ('k, 'v) pfun" is
+"\<lambda> d f x. if (x \<in> d) then Some (f x) else None" .
+    
 definition pcard :: "('a, 'b) pfun \<Rightarrow> nat"
 where "pcard f = card (pdom f)"
 
@@ -98,11 +102,11 @@ where "pfun_subset_eq \<equiv> less_eq"
 instance pfun :: (type, type) semilattice_inf
   by (intro_classes, (transfer, auto simp add: map_le_def dom_def)+)
 
-lemma pfun_subset_eq_least [simp]: 
+lemma pfun_subset_eq_least [simp]:
   "{}\<^sub>p \<subseteq>\<^sub>p f"
   by (transfer, auto)
 
-syntax   
+syntax
   "_PfunUpd"  :: "[('a, 'b) pfun, maplets] => ('a, 'b) pfun" ("_'(_')\<^sub>p" [900,0]900)
   "_Pfun"     :: "maplets => ('a, 'b) pfun"            ("(1{_}\<^sub>p)")
 
@@ -159,7 +163,7 @@ lemma pfun_minus_plus_commute:
 lemma pfun_plus_minus:
   "f \<subseteq>\<^sub>p g \<Longrightarrow> (g - f) + f = g"
   by (transfer, rule ext, auto simp add: map_le_def map_minus_def map_add_def option.case_eq_if)
-  
+
 lemma pfun_minus_common_subset:
   "\<lbrakk> h \<subseteq>\<^sub>p f; h \<subseteq>\<^sub>p g \<rbrakk> \<Longrightarrow> (f - h = g - h) = (f = g)"
   by (transfer, simp add: map_minus_common_subset)
@@ -190,7 +194,7 @@ lemma pfun_app_upd_1 [simp]: "x = y \<Longrightarrow> (f(x \<mapsto> v)\<^sub>p)
   by (transfer, simp)
 
 lemma pfun_app_upd_2 [simp]: "x \<noteq> y \<Longrightarrow> (f(x \<mapsto> v)\<^sub>p)(y)\<^sub>p = f(y)\<^sub>p"
-  by (transfer, simp) 
+  by (transfer, simp)
 
 lemma pfun_upd_add [simp]: "f + g(x \<mapsto> v)\<^sub>p = (f + g)(x \<mapsto> v)\<^sub>p"
   by (transfer, simp)
@@ -212,23 +216,30 @@ lemma pfun_upd_comm_linorder [simp]:
 lemma pfun_app_minus [simp]: "x \<notin> pdom g \<Longrightarrow> (f - g)(x)\<^sub>p = f(x)\<^sub>p"
   by (transfer, auto simp add: map_minus_def)
 
-lemma pfun_upd_minus [simp]: 
-  "x \<notin> pdom g \<Longrightarrow> (f - g)(x \<mapsto> v)\<^sub>p = (f(x \<mapsto> v)\<^sub>p - g)" 
+lemma pfun_app_empty [simp]: "{}\<^sub>p(x)\<^sub>p = undefined"
+  by (transfer, simp)
+
+lemma pfun_app_not_in_dom: 
+  "x \<notin> pdom(f) \<Longrightarrow> f(x)\<^sub>p = undefined"
+  by (transfer, simp)
+
+lemma pfun_upd_minus [simp]:
+  "x \<notin> pdom g \<Longrightarrow> (f - g)(x \<mapsto> v)\<^sub>p = (f(x \<mapsto> v)\<^sub>p - g)"
   by (transfer, auto simp add: map_minus_def)
 
 lemma pdom_member_minus_iff [simp]:
   "x \<notin> pdom g \<Longrightarrow> x \<in> pdom(f - g) \<longleftrightarrow> x \<in> pdom(f)"
   by (transfer, simp add: domIff map_minus_def)
 
-lemma psubseteq_pfun_upd1 [intro]: 
+lemma psubseteq_pfun_upd1 [intro]:
   "\<lbrakk> f \<subseteq>\<^sub>p g; x \<notin> pdom(g) \<rbrakk> \<Longrightarrow> f \<subseteq>\<^sub>p g(x \<mapsto> v)\<^sub>p"
   by (transfer, auto simp add: map_le_def dom_def)
 
-lemma psubseteq_pfun_upd2 [intro]: 
+lemma psubseteq_pfun_upd2 [intro]:
   "\<lbrakk> f \<subseteq>\<^sub>p g; x \<notin> pdom(f) \<rbrakk> \<Longrightarrow> f \<subseteq>\<^sub>p g(x \<mapsto> v)\<^sub>p"
   by (transfer, auto simp add: map_le_def dom_def)
 
-lemma psubseteq_pfun_upd3 [intro]: 
+lemma psubseteq_pfun_upd3 [intro]:
   "\<lbrakk> f \<subseteq>\<^sub>p g; g(x)\<^sub>p = v \<rbrakk> \<Longrightarrow> f \<subseteq>\<^sub>p g(x \<mapsto> v)\<^sub>p"
   by (transfer, auto simp add: map_le_def dom_def)
 
@@ -270,7 +281,7 @@ lemma pdom_pran_res_finite [simp]:
   "finite (pdom f) \<Longrightarrow> finite (pdom (f \<rhd>\<^sub>p A))"
   by (transfer, auto)
 
-lemma pdom_pfun_graph_finite [simp]: 
+lemma pdom_pfun_graph_finite [simp]:
   "finite (pdom f) \<Longrightarrow> finite (pfun_graph f)"
   by (transfer, simp add: finite_dom_graph)
 
@@ -299,17 +310,32 @@ subsection {* Domain restriction laws *}
 lemma pdom_res_zero [simp]: "A \<lhd>\<^sub>p {}\<^sub>p = {}\<^sub>p"
   by (transfer, auto)
 
+lemma pdom_res_empty [simp]:
+  "({} \<lhd>\<^sub>p f) = {}\<^sub>p"
+  by (transfer, auto)
+      
+lemma pdom_res_UNIV [simp]: "UNIV \<lhd>\<^sub>p f = f"
+  by (transfer, auto)
+    
 lemma pdom_res_alt_def: "A \<lhd>\<^sub>p f =  f \<circ>\<^sub>p pId_on A"
   by (transfer, rule ext, auto simp add: restrict_map_def)
 
-lemma pdom_res_upd_in [simp]: 
+lemma pdom_res_upd_in [simp]:
   "k \<in> A \<Longrightarrow> A \<lhd>\<^sub>p f(k \<mapsto> v)\<^sub>p = (A \<lhd>\<^sub>p f)(k \<mapsto> v)\<^sub>p"
   by (transfer, auto)
 
-lemma pdom_res_upd_out [simp]: 
+lemma pdom_res_upd_out [simp]:
   "k \<notin> A \<Longrightarrow> A \<lhd>\<^sub>p f(k \<mapsto> v)\<^sub>p = A \<lhd>\<^sub>p f"
   by (transfer, auto)
+    
+lemma pfun_pdom_antires_upd [simp]:
+  "k \<in> A \<Longrightarrow> ((- A) \<lhd>\<^sub>p m)(k \<mapsto> v)\<^sub>p =  ((- (A - {k})) \<lhd>\<^sub>p m)(k \<mapsto> v)\<^sub>p"
+  by (transfer, simp)
 
+lemma pdom_antires_insert_notin [simp]:
+  "k \<notin> pdom(f) \<Longrightarrow> (- insert k A) \<lhd>\<^sub>p f = (- A) \<lhd>\<^sub>p f"
+  by (transfer, auto simp add: restrict_map_def)
+ 
 lemma pdom_res_override [simp]: "A \<lhd>\<^sub>p (f + g) = (A \<lhd>\<^sub>p f) + (A \<lhd>\<^sub>p g)"
   by (simp add: pdom_res_alt_def pfun_override_dist_comp)
 
@@ -324,7 +350,11 @@ lemma pdom_res_twice [simp]: "A \<lhd>\<^sub>p (B \<lhd>\<^sub>p f) = (A \<inter
 
 lemma pdom_res_comp [simp]: "A \<lhd>\<^sub>p (g \<circ>\<^sub>p f) =  g \<circ>\<^sub>p (A \<lhd>\<^sub>p f)"
   by (simp add: pdom_res_alt_def pfun_comp_assoc)
-  
+
+lemma pdom_res_apply [simp]:
+  "x \<in> A \<Longrightarrow> (A \<lhd>\<^sub>p f)(x)\<^sub>p = f(x)\<^sub>p"
+  by (transfer, auto)
+    
 subsection {* Range restriction laws *}
 
 lemma pran_res_zero [simp]: "{}\<^sub>p \<rhd>\<^sub>p A = {}\<^sub>p"
@@ -365,8 +395,74 @@ lemma pfun_graph_inter: "pfun_graph (f \<inter>\<^sub>p g) = pfun_graph f \<inte
   apply (metis option.discI)+
 done
 
-text {* Hide implementation details for partial functions *}
+subsection {* Entries *}
   
+lemma pfun_entries_empty [simp]: "pfun_entries {} f = {}\<^sub>p"
+  by (transfer, simp)
+
+lemma pfun_entries_apply_1 [simp]: 
+  "x \<in> d \<Longrightarrow> (pfun_entries d f)(x)\<^sub>p = f x"
+  by (transfer, auto)
+
+lemma pfun_entries_apply_2 [simp]: 
+  "x \<notin> d \<Longrightarrow> (pfun_entries d f)(x)\<^sub>p = undefined"
+  by (transfer, auto)
+
+subsection {* Summation *}
+    
+definition pfun_sum :: "('k, 'v::comm_monoid_add) pfun \<Rightarrow> 'v" where
+"pfun_sum f = sum (pfun_app f) (pdom f)"
+    
+lemma pfun_sum_empty [simp]: "pfun_sum {}\<^sub>p = 0"
+  by (simp add: pfun_sum_def)
+
+lemma pfun_sum_upd_1:
+  assumes "finite(pdom(m))" "k \<notin> pdom(m)"
+  shows "pfun_sum (m(k \<mapsto> v)\<^sub>p) = pfun_sum m + v"
+  by (simp_all add: pfun_sum_def assms, metis add.commute assms(2) pfun_app_upd_2 sum.cong)
+
+lemma pfun_sums_upd_2:
+  assumes "finite(pdom(m))"
+  shows "pfun_sum (m(k \<mapsto> v)\<^sub>p) = pfun_sum ((- {k}) \<lhd>\<^sub>p m) + v"
+proof (cases "k \<notin> pdom(m)")
+  case True
+  then show ?thesis 
+    by (simp add: pfun_sum_upd_1 assms)
+next
+  case False
+  then show ?thesis
+    using assms pfun_sum_upd_1[of "((- {k}) \<lhd>\<^sub>p m)" k v]
+    by (simp add: pfun_sum_upd_1)
+qed
+
+lemma pfun_sum_dom_res_insert [simp]: 
+  assumes "x \<in> pdom f" "x \<notin> A" "finite A" 
+  shows "pfun_sum ((insert x A) \<lhd>\<^sub>p f) = f(x)\<^sub>p + pfun_sum (A \<lhd>\<^sub>p f)"
+  using assms by (simp add: pfun_sum_def)
+  
+lemma pfun_sum_pdom_res:
+  fixes f :: "('a,'b::ab_group_add) pfun"
+  assumes "finite(pdom f)"
+  shows "pfun_sum (A \<lhd>\<^sub>p f) = pfun_sum f - (pfun_sum ((- A) \<lhd>\<^sub>p f))"
+proof -
+  have 1:"A \<inter> pdom(f) = pdom(f) - (pdom(f) - A)"
+    by (auto)
+  show ?thesis
+    apply (simp add: pfun_sum_def)
+    apply (subst 1)
+    apply (subst sum_diff)
+    apply (auto simp add: sum_diff Diff_subset Int_commute boolean_algebra_class.diff_eq assms)
+  done
+qed
+  
+lemma pfun_sum_pdom_antires [simp]:
+  fixes f :: "('a,'b::ab_group_add) pfun"
+  assumes "finite(pdom f)"
+  shows "pfun_sum ((- A) \<lhd>\<^sub>p f) = pfun_sum f - pfun_sum (A \<lhd>\<^sub>p f)"
+  by (subst pfun_sum_pdom_res, simp_all add: assms)
+  
+text {* Hide implementation details for partial functions *}
+
 lifting_update pfun.lifting
 lifting_forget pfun.lifting
 
