C-verifier/src/Midend-IVL/Isabelle-UTP/utp/utp_rel.thy
@@ -14,11 +14,19 @@ begin
 type_synonym '\<alpha> cond      = "'\<alpha> upred"
 type_synonym ('\<alpha>, '\<beta>) rel = "('\<alpha> \<times> '\<beta>) upred"
 type_synonym '\<alpha> hrel      = "('\<alpha> \<times> '\<alpha>) upred"
+type_synonym ('a, '\<alpha>) hexpr = "('a, '\<alpha> \<times> '\<alpha>) uexpr"
 
 translations
   (type) "('\<alpha>, '\<beta>) rel" <= (type) "('\<alpha> \<times> '\<beta>) upred"
-
-subsection{*SKIP*}
+  
+text {* We set up some overloaded constants for sequential composition and the identity in case
+  we want to overload their definitions later. *}
+  
+consts
+  useq   :: "'a \<Rightarrow> 'b \<Rightarrow> 'c" (infixr ";;" 71)
+  uskip  :: "'a" ("II")
+ 
+subsection{*SKIP*}                                                     
 
 
 definition skip_ra :: "('\<beta>, '\<alpha>) lens \<Rightarrow>'\<alpha> hrel" where
@@ -35,17 +43,18 @@ lift_definition assigns_r :: "'\<alpha> usubst \<Rightarrow> '\<alpha> hrel" ("\
 
 definition skip_r :: "'\<alpha> hrel" where
 [urel_defs]:"skip_r = assigns_r id"
-
+adhoc_overloading
+  uskip skip_r
 subsection{*Assign*}
 
 definition assigns_ra :: "'\<alpha> usubst \<Rightarrow> ('\<beta>, '\<alpha>) lens \<Rightarrow> '\<alpha> hrel" ("\<langle>_\<rangle>\<^bsub>_\<^esub>") where
 "\<langle>\<sigma>\<rangle>\<^bsub>a\<^esub> = (\<lceil>\<sigma>\<rceil>\<^sub>s \<dagger> II\<^bsub>a\<^esub>)"
 
-abbreviation assign_r :: "('t, '\<alpha>) uvar \<Rightarrow> ('t, '\<alpha>) uexpr \<Rightarrow> '\<alpha> hrel"  where 
+abbreviation assign_r :: "('t \<Longrightarrow> '\<alpha>) \<Rightarrow> ('t, '\<alpha>) uexpr \<Rightarrow> '\<alpha> hrel"  where 
   "assign_r v expr \<equiv> assigns_r [v \<mapsto>\<^sub>s expr]"
 
 abbreviation assign_2_r ::
-  "('t1, '\<alpha>) uvar \<Rightarrow> ('t2, '\<alpha>) uvar \<Rightarrow> ('t1, '\<alpha>) uexpr \<Rightarrow> ('t2, '\<alpha>) uexpr \<Rightarrow> '\<alpha> hrel" where 
+  "('t1 \<Longrightarrow> '\<alpha>) \<Rightarrow> ('t2 \<Longrightarrow> '\<alpha>) \<Rightarrow> ('t1, '\<alpha>) uexpr \<Rightarrow> ('t2, '\<alpha>) uexpr \<Rightarrow> '\<alpha> hrel" where 
   "assign_2_r x y u v \<equiv> assigns_r [x \<mapsto>\<^sub>s u, y \<mapsto>\<^sub>s v]"
 
 subsection{*Conditional*}
@@ -58,34 +67,25 @@ subsection{*Sequential composition*}
 
 lift_definition seqr::"('\<alpha>, '\<beta>) rel \<Rightarrow> ('\<beta>, '\<gamma>) rel \<Rightarrow> ('\<alpha>, '\<gamma>) rel"  is
   "\<lambda> P Q r. r \<in> ({p. P p} O {q. Q q})" .
+ adhoc_overloading
+  useq seqr
+  
+text {* We also set up a homogeneous sequential composition operator, and versions of @{term true}
+  and @{term false} that are explicitly typed by a homogeneous alphabet. *}
 
-lift_definition conv_r :: "('a, '\<alpha> \<times> '\<beta>) uexpr \<Rightarrow> ('a, '\<beta> \<times> '\<alpha>) uexpr" ("_\<^sup>-" [999] 999)
-is "\<lambda> e (b1, b2). e (b2, b1)" .
+abbreviation seqh :: "'\<alpha> hrel \<Rightarrow> '\<alpha> hrel \<Rightarrow> '\<alpha> hrel" (infixr ";;\<^sub>h" 71) where
+"seqh P Q \<equiv> (P ;; Q)"
 
-subsection{*Syntax setup*}
+text {* We set up iterated sequential composition which iterates an indexed predicate over the
+  elements of a list. *}
+  
+definition seqr_iter :: "'a list \<Rightarrow> ('a \<Rightarrow> 'b hrel) \<Rightarrow> 'b hrel" where
+[urel_defs]: "seqr_iter xs P = foldr (\<lambda> i Q. P(i) ;; Q) xs II"    
 
-nonterminal
-  svid_list and uexpr_list
+abbreviation conv_r :: "('a, '\<alpha> \<times> '\<beta>) uexpr \<Rightarrow> ('a, '\<beta> \<times> '\<alpha>) uexpr" ("_\<^sup>-" [999] 999)
+where "conv_r e \<equiv> e \<oplus>\<^sub>p swap\<^sub>L"
+  
 
-syntax
-  "_svid_unit"  :: "svid \<Rightarrow> svid_list" ("_")
-  "_svid_list"  :: "svid \<Rightarrow> svid_list \<Rightarrow> svid_list" ("_,/ _")
-  "_uexpr_unit" :: "('a, '\<alpha>) uexpr \<Rightarrow> uexpr_list" ("_" [40] 40)
-  "_uexpr_list" :: "('a, '\<alpha>) uexpr \<Rightarrow> uexpr_list \<Rightarrow> uexpr_list" ("_,/ _" [40,40] 40)
-  "_assignment" :: "svid_list \<Rightarrow> uexprs \<Rightarrow> '\<alpha> hrel"  ("_ :== _ " [60, 60] 52)
-  "_mk_usubst"  :: "svid_list \<Rightarrow> uexprs \<Rightarrow> '\<alpha> usubst"
-
-translations
-  "_mk_usubst \<sigma> (_svid_unit x) v" == "\<sigma>(&x \<mapsto>\<^sub>s v)"
-  "_mk_usubst \<sigma> (_svid_list x xs) (_uexprs v vs)" == "(_mk_usubst (\<sigma>(&x \<mapsto>\<^sub>s v)) xs vs)"
-  "_assignment xs vs" => "CONST assigns_r (_mk_usubst (CONST id) xs vs)"
-  "x :== v" <= "CONST assigns_r (CONST subst_upd (CONST id) (CONST svar x) v)"
-  "x :== v" <= "CONST assigns_r (CONST subst_upd (CONST id) x v)"
-  "x,y :== u,v" <= "CONST assigns_r (CONST subst_upd (CONST subst_upd (CONST id) (CONST svar x) u) (CONST svar y) v)"
-
-adhoc_overloading
-  useq seqr and
-  uskip skip_r
 
 subsection{*While-loop*}
 text{*In order to specify while loops we need a concept that refers to the result of the execution
@@ -110,7 +110,7 @@ declare while_def [urel_defs]
 subsection{*While-loop inv*}
 text {* While loops with invariant decoration *}
 
-definition while_inv :: "'\<alpha> cond \<Rightarrow> '\<alpha> cond \<Rightarrow> '\<alpha> hrel \<Rightarrow> '\<alpha> hrel" ("while _ invr _ do _ od" 70) where
+definition while_inv :: "'\<alpha> cond \<Rightarrow> '\<alpha> cond \<Rightarrow> '\<alpha> hrel \<Rightarrow> '\<alpha> hrel" ("while _ invr _ do _ od" 71) where
 "while b invr p do S od = while\<^sup>\<top> b do S od"
 
 subsection{*assert and assume*}
@@ -121,9 +121,32 @@ definition rassume :: "'\<alpha> upred \<Rightarrow> '\<alpha> hrel" ("_\<^sup>\
 definition rassert :: "'\<alpha> upred \<Rightarrow> '\<alpha> hrel" ("_\<^sub>\<bottom>" [999] 999) where
 [urel_defs]: "rassert c = II \<triangleleft> c \<triangleright>\<^sub>r true"
 
-subsection{*throw*} 
-text{*To model exceptions we need to use the flag OK from UTP.
-      It is a way to capture the termination or non termination of a program.*}
+text {* Homogeneous relations form a quantale. This allows us to import a large number of laws
+        from Struth and Armstrong's Kleene Algebra theory~\cite{Armstrong2015}. *}
+
+abbreviation truer :: "'\<alpha> hrel" ("true\<^sub>h") where
+"truer \<equiv> true"
+
+abbreviation falser :: "'\<alpha> hrel" ("false\<^sub>h") where
+"falser \<equiv> false"
+
+text {* We next describe frames and antiframes with the help of lenses. A frame states that $P$
+  defines the behaviour of all variables not in $a$, and all those in $a$ remain the same. An
+  antiframe describes the converse: all variables in $a$ are specified by $P$, and all other
+  variables remain the same. For more information please see \cite{Morgan90a}.*}
+
+definition frame :: "('a \<Longrightarrow> '\<alpha>) \<Rightarrow> '\<alpha> hrel \<Rightarrow> '\<alpha> hrel" where
+[urel_defs]: "frame a P = (\<^bold>\<exists> st \<bullet> P\<lbrakk>\<guillemotleft>st\<guillemotright>/$\<Sigma>\<acute>\<rbrakk> \<and> $\<Sigma>\<acute> =\<^sub>u \<guillemotleft>st\<guillemotright> \<oplus> $\<Sigma> on &a)"
+
+definition antiframe :: "('a \<Longrightarrow> '\<alpha>) \<Rightarrow> '\<alpha> hrel \<Rightarrow> '\<alpha> hrel" where
+[urel_defs]: "antiframe a P = (\<^bold>\<exists> st \<bullet> P\<lbrakk>\<guillemotleft>st\<guillemotright>/$\<Sigma>\<acute>\<rbrakk> \<and> $\<Sigma>\<acute> =\<^sub>u $\<Sigma> \<oplus> \<guillemotleft>st\<guillemotright> on &a)"
+
+text {* The nameset operator can be used to hide a portion of the after-state that lies outside
+  the lens $a$. It can be useful to partition a relation's variables in order to conjoin it
+  with another relation. *}
+
+definition nameset :: "('a \<Longrightarrow> '\<alpha>) \<Rightarrow> '\<alpha> hrel \<Rightarrow> '\<alpha> hrel" where
+[urel_defs]: "nameset a P = (P \<restriction>\<^sub>v {$\<Sigma>,$a\<acute>})" 
 
 subsection{*block*}
 text{*Block is used to model scoping. This feature can be used to introduce local variables and 
@@ -149,6 +172,64 @@ definition block :: "('a, 'c) rel \<Rightarrow> ('c, 'd) rel  \<Rightarrow> ('a 
              Abs_uexpr (\<lambda>(t, t').\<lbrakk>restore (s, s') (t, t');; return(s, s') (t, t')\<rbrakk>\<^sub>e (t, t'))\<rbrakk>\<^sub>e (s, s'))" 
 
 
+
+subsection {* Syntax Translations Setup*}
+    
+syntax
+  -- {* Alternative traditional conditional syntax *}
+  "_utp_if" :: "logic \<Rightarrow> logic \<Rightarrow> logic \<Rightarrow> logic" ("(if\<^sub>u (_)/ then (_)/ else (_))" [0, 0, 71] 71)
+  -- {* Iterated sequential composition *}
+  "_seqr_iter" :: "pttrn \<Rightarrow> 'a list \<Rightarrow> '\<sigma> hrel \<Rightarrow> '\<sigma> hrel" ("(3;; _ : _ \<bullet>/ _)" [0, 0, 10] 10)
+  -- {* Single and multiple assignement *}
+  "_assignment"     :: "svids \<Rightarrow> uexprs \<Rightarrow> '\<alpha> hrel"  ("'(_') :== '(_')")  
+  "_assignment"     :: "svids \<Rightarrow> uexprs \<Rightarrow> '\<alpha> hrel"  (infixr ":==" 72)
+  -- {* Indexed assignment *}
+  "_assignment_upd" :: "svid \<Rightarrow> logic \<Rightarrow> logic \<Rightarrow> logic" ("(_[_] :==/ _)" [73, 0, 0] 72)
+  -- {* Substitution constructor *}
+  "_mk_usubst"      :: "svids \<Rightarrow> uexprs \<Rightarrow> '\<alpha> usubst"
+  -- {* Alphabetised skip *}
+  "_skip_ra"        :: "salpha \<Rightarrow> logic" ("II\<^bsub>_\<^esub>")
+  -- {* Frame *}
+  "_frame"          :: "salpha \<Rightarrow> logic \<Rightarrow> logic" ("_:\<lbrakk>_\<rbrakk>" [79,0] 80)
+  -- {* Antiframe *}
+  "_antiframe"      :: "salpha \<Rightarrow> logic \<Rightarrow> logic" ("_:[_]" [99,0] 100)
+  -- {* Nameset *}
+  "_nameset"        :: "salpha \<Rightarrow> logic \<Rightarrow> logic" ("ns _ \<bullet> _" [0,999] 999)
+  
+translations
+  "_utp_if b P Q" => "P \<triangleleft> b \<triangleright>\<^sub>r Q"
+  ";; x : l \<bullet> P" \<rightleftharpoons> "(CONST seqr_iter) l (\<lambda>x. P)"
+  "_mk_usubst \<sigma> (_svid_unit x) v" \<rightleftharpoons> "\<sigma>(&x \<mapsto>\<^sub>s v)"
+  "_mk_usubst \<sigma> (_svid_list x xs) (_uexprs v vs)" \<rightleftharpoons> "(_mk_usubst (\<sigma>(&x \<mapsto>\<^sub>s v)) xs vs)"
+  "_assignment xs vs" => "CONST assigns_r (_mk_usubst (CONST id) xs vs)"
+  "x :== v" <= "CONST assigns_r (CONST subst_upd (CONST id) (CONST svar x) v)"
+  "x :== v" <= "CONST assigns_r (CONST subst_upd (CONST id) x v)"
+  "x,y :== u,v" <= "CONST assigns_r (CONST subst_upd (CONST subst_upd (CONST id) (CONST svar x) u) (CONST svar y) v)"
+  -- {* Indexed assignment uses the overloaded collection update function \emph{uupd}. *}
+  "x [k] :== v" => "x :== &x(k \<mapsto> v)\<^sub>u"
+  "_skip_ra v" \<rightleftharpoons> "CONST skip_ra v"
+  "_frame x P" \<rightleftharpoons> "CONST frame x P"
+  "_antiframe x P" \<rightleftharpoons> "CONST antiframe x P"
+  "_nameset x P" \<rightleftharpoons> "CONST nameset x P"
+
+ text {* The following code sets up pretty-printing for homogeneous relational expressions. We cannot 
+  do this via the ``translations'' command as we only want the rule to apply when the input and output
+  alphabet types are the same. The code has to deconstruct a @{typ "('a, '\<alpha>) uexpr"} type, determine 
+  that it is relational (product alphabet), and then checks if the types \emph{alpha} and \emph{beta} 
+  are the same. If they are, the type is printed as a \emph{hexpr}. Otherwise, we have no match. 
+  We then set up a regular translation for the \emph{hrel} type that uses this. *}
+  
+print_translation {*
+let
+fun tr' ctx [ a
+            , Const (@{type_syntax "prod"},_) $ alpha $ beta ] = 
+  if (alpha = beta) 
+    then Syntax.const @{type_syntax "hexpr"} $ a $ alpha
+    else raise Match;
+in [(@{type_syntax "uexpr"},tr')]
+end
+*} 
+  
 subsection {* Program values *}
 
 abbreviation prog_val :: "'\<alpha> hrel \<Rightarrow> ('\<alpha> hrel, '\<alpha>) uexpr" ("\<lbrace>|_|\<rbrace>\<^sub>u")
@@ -160,25 +241,24 @@ is "\<lambda> P b. P (fst b) b" .
 lemma call_prog_val: "call \<lbrace>|P|\<rbrace>\<^sub>u = P"
   by (simp add: call_def urel_defs lit.rep_eq Rep_uexpr_inverse)
 
-notation (latex)
+(*notation (latex)
   skip_r  ("\<SKIP>") and
   cond  ("\<IF> _ \<THEN> _ \<ELSE> _"  60) and
-  while  ("\<WHILE> _ \<DO> _ \<OD>"  60)
+  while  ("\<WHILE> _ \<DO> _ \<OD>"  60)*)
 
 subsection {*Props *}
 
-text {* We describe some properties of relations *}
+text {* We describe some properties of relations, including functional and injective relations. *}
 
 definition ufunctional :: "('a, 'b) rel \<Rightarrow> bool"
-where "ufunctional R \<longleftrightarrow> II \<sqsubseteq> R\<^sup>- ;; R"
-
-declare ufunctional_def [urel_defs]
+where [urel_defs]: "ufunctional R \<longleftrightarrow> II \<sqsubseteq> R\<^sup>- ;; R"
 
 definition uinj :: "('a, 'b) rel \<Rightarrow> bool"
-where "uinj R \<longleftrightarrow> II \<sqsubseteq> R ;; R\<^sup>-"
+where [urel_defs]: "uinj R \<longleftrightarrow> II \<sqsubseteq> R ;; R\<^sup>-"
 
-declare uinj_def [urel_defs]
+-- {* Configuration for UTP tactics (see @{theory utp_tactics}). *}
 
+update_uexpr_rep_eq_thms -- {* Reread @{text rep_eq} theorems. *}
 text {* A test is like a precondition, except that it identifies to the postcondition. It
         forms the basis for Kleene Algebra with Tests (KAT). *}
 
@@ -190,14 +270,8 @@ declare skip_r_def [urel_defs]
 
 text {* We implement a poor man's version of alphabet restriction that hides a variable within a relation *}
 
-definition rel_var_res :: "'\<alpha> hrel \<Rightarrow> ('a, '\<alpha>) uvar \<Rightarrow> '\<alpha> hrel" (infix "\<restriction>\<^sub>\<alpha>" 80) where
-"P \<restriction>\<^sub>\<alpha> x = (\<exists> $x \<bullet> \<exists> $x\<acute> \<bullet> P)"
-
-declare rel_var_res_def [urel_defs]
-
--- {* Configuration for UTP tactics (see @{theory utp_tactics}). *}
-
-update_uexpr_rep_eq_thms -- {* Reread @{text rep_eq} theorems. *}
+definition rel_var_res :: "'\<alpha> hrel \<Rightarrow> ('a \<Longrightarrow> '\<alpha>)  \<Rightarrow> '\<alpha> hrel" (infix "\<restriction>\<^sub>\<alpha>" 80) where
+[urel_defs]:"P \<restriction>\<^sub>\<alpha> x = (\<exists> $x \<bullet> \<exists> $x\<acute> \<bullet> P)"
 
 lemma Rep_inverse[code]:"Rep_uexpr (Abs_uexpr x) = x" 
 by rel_auto
