C-verifier/src/Midend-IVL/Isabelle-UTP/utp/utp_urel_setup.thy
@@ -1,21 +1,31 @@
 section {* UTP variables *}
 
 theory utp_urel_setup
-  imports utp_lift utp_tactics
+  imports utp_lift utp_tactics utp_recursion
 begin
 (*tactics are in utp_tactics*)
-consts
-  useq   :: "'a \<Rightarrow> 'b \<Rightarrow> 'c" (infixr ";;" 51)
-  uskip  :: "'a" ("II")
 
-definition in\<alpha> :: "('\<alpha>, '\<alpha> \<times> '\<beta>) uvar" where
-"in\<alpha> = \<lparr> lens_get = fst, lens_put = \<lambda> (A, A') v. (v, A') \<rparr>"
+text {* An alphabetised relation is simply a predicate whose state-space is a product type. In this
+  theory we construct the core operators of the relational calculus, and prove a libary of 
+  associated theorems, based on Chapters 2 and 5 of the UTP book~\cite{Hoare&98}. *}
+  
+subsection {* Relational Alphabets *}
+  
+text {* We set up convenient syntax to refer to the input and output parts of the alphabet, as is
+  common in UTP. Since we are in a product space, these are simply the lenses @{term "fst\<^sub>L"} and
+  @{term "snd\<^sub>L"}. *}
+  
+definition in\<alpha> :: "('\<alpha> \<Longrightarrow> '\<alpha> \<times> '\<beta>)" where
+[lens_defs]: "in\<alpha> = fst\<^sub>L"
 
-definition out\<alpha> :: "('\<beta>, '\<alpha> \<times> '\<beta>) uvar" where
-"out\<alpha> = \<lparr> lens_get = snd, lens_put = \<lambda> (A, A') v. (A, v) \<rparr>"
+definition out\<alpha> :: "('\<beta> \<Longrightarrow> '\<alpha> \<times> '\<beta>)" where
+[lens_defs]: "out\<alpha> = snd\<^sub>L"
 
-declare in\<alpha>_def [urel_defs]
-declare out\<alpha>_def [urel_defs]
+lemma in\<alpha>_uvar [simp]: "vwb_lens in\<alpha>"
+  by (unfold_locales, auto simp add: in\<alpha>_def)
+
+lemma out\<alpha>_uvar [simp]: "vwb_lens out\<alpha>"
+  by (unfold_locales, auto simp add: out\<alpha>_def)
 
 lemma var_in_alpha [simp]: "x ;\<^sub>L in\<alpha> = ivar x"
   by (simp add: fst_lens_def in\<alpha>_def in_var_def)
@@ -23,25 +33,37 @@ lemma var_in_alpha [simp]: "x ;\<^sub>L in\<alpha> = ivar x"
 lemma var_out_alpha [simp]: "x ;\<^sub>L out\<alpha> = ovar x"
   by (simp add: out\<alpha>_def out_var_def snd_lens_def)
 
+lemma drop_pre_inv [simp]: "\<lbrakk> out\<alpha> \<sharp> p \<rbrakk> \<Longrightarrow> \<lceil>\<lfloor>p\<rfloor>\<^sub><\<rceil>\<^sub>< = p"
+  by (pred_simp)
+
+lemma usubst_lookup_ivar_unrest [usubst]:
+  "in\<alpha> \<sharp> \<sigma> \<Longrightarrow> \<langle>\<sigma>\<rangle>\<^sub>s (ivar x) = $x"
+  by (rel_simp, metis fstI)
+
+lemma usubst_lookup_ovar_unrest [usubst]:
+  "out\<alpha> \<sharp> \<sigma> \<Longrightarrow> \<langle>\<sigma>\<rangle>\<^sub>s (ovar x) = $x\<acute>"
+  by (rel_simp, metis sndI)
+    
 lemma out_alpha_in_indep [simp]:
   "out\<alpha> \<bowtie> in_var x" "in_var x \<bowtie> out\<alpha>"
-  by (simp_all add: in_var_def out\<alpha>_def lens_indep_def fst_lens_def lens_comp_def)
+  by (simp_all add: in_var_def out\<alpha>_def lens_indep_def fst_lens_def snd_lens_def lens_comp_def)
 
 lemma in_alpha_out_indep [simp]:
   "in\<alpha> \<bowtie> out_var x" "out_var x \<bowtie> in\<alpha>"
   by (simp_all add: in_var_def in\<alpha>_def lens_indep_def fst_lens_def lens_comp_def)
 
-text {* The alphabet of a relation consists of the input and output portions *}
-
-lemma alpha_in_out:
-  "\<Sigma> \<approx>\<^sub>L in\<alpha> +\<^sub>L out\<alpha>"
-  by (metis fst_lens_def fst_snd_id_lens in\<alpha>_def lens_equiv_refl out\<alpha>_def snd_lens_def)
-
+text {* The following two functions lift a predicate substitution to a relational one. *}
+    
 abbreviation usubst_rel_lift :: "'\<alpha> usubst \<Rightarrow> ('\<alpha> \<times> '\<beta>) usubst" ("\<lceil>_\<rceil>\<^sub>s") where
 "\<lceil>\<sigma>\<rceil>\<^sub>s \<equiv> \<sigma> \<oplus>\<^sub>s in\<alpha>"
 
 abbreviation usubst_rel_drop :: "('\<alpha> \<times> '\<alpha>) usubst \<Rightarrow> '\<alpha> usubst" ("\<lfloor>_\<rfloor>\<^sub>s") where
 "\<lfloor>\<sigma>\<rfloor>\<^sub>s \<equiv> \<sigma> \<restriction>\<^sub>s in\<alpha>"
+    
+text {* The alphabet of a relation then consists wholly of the input and output portions. *}
 
+lemma alpha_in_out:
+  "\<Sigma> \<approx>\<^sub>L in\<alpha> +\<^sub>L out\<alpha>"
+  by (simp add: fst_snd_id_lens in\<alpha>_def lens_equiv_refl out\<alpha>_def)
 
 end
